cleanup

dijkstra/verif_dijkstra.v
@@ -1220,6 +1220,164 @@ Definition dijk_forloop_break_inv g sh src dist_ptr prev_ptr priq_ptr graph_ptr 
               (pointer_val_val dist_ptr);
       DijkGraph sh CompSpecs g (pointer_val_val graph_ptr)).
 
+Definition dijk_inner_forloop_inv (g: DijkGG) sh src priq dist_ptr prev_ptr priq_ptr graph_ptr :=
+  EX i : Z,
+  EX prev' : list V,
+  EX priq' : list V,
+  EX dist' : list V,
+  EX popped' : list V,
+  let u :=
+      find priq (fold_right Z.min (hd 0 priq) priq) 0 in
+  PROP (
+      (* inv_popped is not affected *)
+      forall dst,
+        vvalid g dst ->
+        inv_popped g src popped' prev' dist' dst;
+    
+    (* and, because we broke out when dist[u] = inf,
+       we know that none of the popped items have dist inf.
+       Essentially, the first disjunct of inv_popped
+       is impossible inside the for loop.
+     *)
+    forall dst,
+      vvalid g dst ->
+      In dst popped' ->
+      Znth dst dist' <> inf;
+    
+    (* inv_unpopped is restored for those vertices
+       that the for loop has scanned and repaired *)
+    forall dst,
+      0 <= dst < i ->
+      inv_unpopped g src popped' prev' dist' dst;
+    
+    (* a weaker version of inv_popped is
+       true for those vertices that the
+       for loop has not yet scanned *)
+    forall dst,
+      i <= dst < SIZE ->
+      inv_unpopped_weak g src popped' prev' dist' dst u;
+    
+    (* similarly for inv_unseen,
+       the invariant has been
+       restored until i:
+       u has been taken into account *)
+    forall dst,
+      0 <= dst < i ->
+      inv_unseen g popped' dist' dst;
+    
+    (* and a weaker version of inv_unseen is
+       true for those vertices that the
+       for loop has not yet scanned *)
+    forall dst,
+      i <= dst < SIZE ->
+      inv_unseen_weak g popped' dist' dst u;
+    (* further, some useful facts about src... *)
+    Znth src dist' = 0;
+    Znth src prev' = src;
+    (* Znth src priq' <> inf; *)
+    
+    (* a useful fact about u *)
+    In u popped';
+    
+    (* A fact about the relationship b/w 
+       dist and priq arrays *)
+    forall dst,
+      vvalid g dst ->
+      ~ In dst popped' ->
+      Znth dst priq' = Znth dst dist';
+    
+    (* and ranges of the three arrays *)
+    inrange_prev prev';
+    inrange_priq priq';
+    inrange_dist dist')
+       
+  LOCAL (temp _u (Vint (Int.repr u));
+        temp _dist (pointer_val_val dist_ptr);
+        temp _prev (pointer_val_val prev_ptr);
+        temp _src (Vint (Int.repr src));
+        lvar _pq (tarray tint SIZE) priq_ptr;
+        temp _graph (pointer_val_val graph_ptr))
+  SEP (data_at Tsh
+               (tarray tint SIZE)
+               (map Vint (map Int.repr prev'))
+               (pointer_val_val prev_ptr);
+      data_at Tsh
+              (tarray tint SIZE)
+              (map Vint (map Int.repr priq')) priq_ptr;
+      data_at Tsh
+              (tarray tint SIZE)
+              (map Vint (map Int.repr dist'))
+              (pointer_val_val dist_ptr);
+      DijkGraph sh CompSpecs g (pointer_val_val graph_ptr)).
+
+Lemma inv_unpopped_weak_add_unpopped:
+  forall (g: DijkGG) prev dist popped src u dst,
+    dijkstra_correct g src popped prev dist ->
+    ~ In u popped ->
+    vvalid g dst ->
+    inv_unpopped_weak g src (u :: popped) prev dist dst u.
+Proof.
+  (* Any vertex that is
+     "seen but not popped"
+     is that way without the benefit of unpopped vertices.
+     We will be asked to provide a locally optimal   
+     path to such a dst, and we will simply provide the 
+     old one best-known path
+   *)
+  intros.
+  unfold inv_unpopped_weak. intros.
+  apply not_in_cons in H2; destruct H2 as [_ ?].
+  destruct (H dst H1) as [_ [? _]].
+  specialize (H4 H2 H3) as
+      [? | [? [? [? [? [? [? ?]]]]]]]; [left | right]; trivial.
+  remember (Znth dst prev) as mom.
+  
+  assert (evalid g (mom, dst)). {
+    rewrite (evalid_meaning g). split.
+    apply (edge_representable).
+    intro. rewrite <- H11 in H7. 
+    apply Zlt_not_le in H7.
+    apply H7; reflexivity.
+  }
+  
+  assert (Znth mom dist < inf) by
+      (pose proof (valid_edge_bounds g _ H11); ulia).
+  
+  destruct (popped_noninf_has_path H H6 H12) as [p2mom [? [? ?]]]; trivial.
+            
+  (* Several of the proof obligations
+     fall away easily, and those that remain
+     boil down to showing that
+     u was not involved in this
+     locally optimal path.
+   *)
+  assert (mom <> u). {
+    intro contra. rewrite contra in *. apply H0; trivial. 
+  }
+  
+  split3; [|split3; [| |split3; [| |split]]|]; trivial.
+  1: simpl; right; trivial.
+  intros.
+  apply H10; trivial.
+  simpl in H19; destruct H19; trilia.
+Qed.
+
+Lemma inv_unseen_weak_add_unpopped:
+  forall (g : DijkGG) prev dist popped src u dst,
+    dijkstra_correct g src popped prev dist ->
+    ~ In u popped ->
+    vvalid g dst ->
+    inv_unseen_weak g (u :: popped) dist dst u.
+Proof.
+  intros.
+  unfold inv_unseen_weak. intros.
+  assert (e: dst <> u) by (simpl in H2; lia).
+  apply not_in_cons in H2; destruct H2 as [_ ?].
+  destruct (H dst H1) as [_ [_ ?]].
+  apply H7; trivial.
+  simpl in H5; destruct H5; [lia | trivial].
+Qed.
+
 Lemma list_repeat1:
   forall {A} (a: A),
     list_repeat (Z.to_nat 1) a = [a].
@@ -1259,6 +1417,86 @@ Proof.
   apply (vvalid_meaning g) in H0. 
   rewrite upd_Znth_diff in H2; trivial.
   rewrite Znth_list_repeat_inrange in H2; ulia.
+Qed.
+
+Lemma In_links_snd_In_path:
+  forall (g: DijkGG) step path,
+    In step (snd path) ->
+    In_path g (snd step) path.
+Proof.
+  intros. unfold In_path. right.
+  exists step. split; trivial.
+  right. rewrite (edge_dst_snd g); trivial.
+Qed.
+
+Lemma In_links_fst_In_path:
+  forall (g: DijkGG) step path,
+    In step (snd path) ->
+    In_path g (fst step) path.
+Proof.
+  intros. unfold In_path. right.
+  exists step. split; trivial.
+  left. rewrite (edge_src_fst g); trivial.
+Qed.
+  
+Lemma inv_popped_newcost:
+  forall (g: DijkGG) src dst u i newcost popped prev dist,
+    vvalid g i ->
+    vvalid g dst ->
+    (forall dst : Z,
+        vvalid g dst ->
+        inv_popped g src popped prev dist dst) ->
+    (forall dst : Z,
+        vvalid g dst ->
+        In dst popped ->
+        Znth dst dist <> inf) ->
+    Zlength prev = SIZE ->
+    Zlength dist = SIZE ->
+    ~ In i popped ->
+    inv_popped g src popped
+               (upd_Znth i prev u)
+               (upd_Znth i dist newcost) dst.
+Proof.
+  intros.
+  unfold inv_popped; intros.
+  assert (n: dst <> i). {
+    intro. subst dst. apply H5; trivial.
+  }
+  assert (0 <= dst < SIZE). {
+  apply (vvalid_meaning g) in H0; ulia.
+  }
+  assert (0 <= i < SIZE). {
+    apply (vvalid_meaning g) in H; ulia.
+  }
+  repeat rewrite upd_Znth_diff; try ulia.
+  destruct (H1 dst H0 H6)
+    as [[? ?] | [p2dst [? [? ?]]]]; [exfalso | right].
+  1: specialize (H2 _ H0 H6); ulia.
+  exists p2dst. split3; trivial.
+  - destruct H9 as [? [? [? [? ?]]]].
+    split3; [| | split3]; trivial.
+    1: rewrite upd_Znth_diff; ulia.
+    rewrite Forall_forall; intros.
+    pose proof (In_links_snd_In_path g _ _ H16).
+    specialize (H10 _ H17). destruct H10.
+    rewrite Forall_forall in H15. specialize (H15 _ H16).
+    assert (snd x <> i). {
+      intro contra. unfold V in *.
+      rewrite contra in *. apply H5; ulia.
+    }
+    unfold V in *.
+    rewrite upd_Znth_diff; try lia.
+    rewrite H3, <- (vvalid_meaning g); trivial.
+    apply (valid_path_valid _ p2dst); trivial.
+  - unfold path_in_popped. intros.
+    specialize (H10 _ H12). destruct H10.
+    assert (step <> i). {
+      intro contra. subst step. apply H5; ulia.
+    }
+    split; trivial. unfold V in *.
+    rewrite upd_Znth_diff; trivial; [|ulia].
+    rewrite H4, <- (vvalid_meaning g); trivial.
+    destruct H9. apply (valid_path_valid _ p2dst); trivial.
 Qed.
 
 (** PROOF BEGINS **)
@@ -1597,97 +1835,8 @@ Proof.
          *)
         forward_for_simple_bound
           SIZE
-          (EX i : Z,
-           EX prev' : list V,
-           EX priq' : list V,
-           EX dist' : list V,
-           EX popped' : list V,
-           PROP (
-               (* inv_popped is not affected *)
-               forall dst,
-                 vvalid g dst ->
-                 inv_popped g src popped' prev'
-                            dist' dst;
-
-                 (* and, because we broke out when dist[u] = inf,
-                    we know that none of the popped items have dist inf.
-                    Essentially, the first disjunct of inv_popped
-                    is impossible inside the for loop.
-                  *)
-               forall dst,
-                 vvalid g dst ->
-                 In dst popped' ->
-                 Znth dst dist' <> inf;
-                 
-                 (* inv_unpopped is restored for those vertices
-                 that the for loop has scanned and repaired *)
-               forall dst,
-                 0 <= dst < i ->
-                 inv_unpopped g src popped' prev'
-                              dist' dst;
-                 
-                 (* a weaker version of inv_popped is
-                    true for those vertices that the
-                    for loop has not yet scanned *)
-               forall dst,
-                 i <= dst < SIZE ->
-                 inv_unpopped_weak g src popped' prev'
-                                   dist' dst u;
-                       
-                   (* similarly for inv_unseen,
-                      the invariant has been
-                      restored until i:
-                      u has been taken into account *)
-               forall dst,
-                 0 <= dst < i ->
-                 inv_unseen g popped'
-                            dist' dst;
-
-                 (* and a weaker version of inv_unseen is
-                    true for those vertices that the
-                    for loop has not yet scanned *)
-               forall dst,
-                 i <= dst < SIZE ->
-                 inv_unseen_weak g popped' 
-                                 dist' dst u;
-                 (* further, some useful facts about src... *)
-                 Znth src dist' = 0;
-                 Znth src prev' = src;
-                 (* Znth src priq' <> inf; *)
-                 
-                 (* a useful fact about u *)
-                 In u popped';
-                 
-                 (* A fact about the relationship b/w 
-                    dist and priq arrays *)
-               forall dst,
-                 vvalid g dst ->
-                 ~ In dst popped' ->
-                 Znth dst priq' = Znth dst dist';
-                       
-                 (* and ranges of the three arrays *)
-                 inrange_prev prev';
-                 inrange_priq priq';
-                 inrange_dist dist')
-                
-                 LOCAL (temp _u (Vint (Int.repr u));
-                        temp _dist (pointer_val_val dist_ptr);
-                        temp _prev (pointer_val_val prev_ptr);
-                        temp _src (Vint (Int.repr src));
-                        lvar _pq (tarray tint SIZE) priq_ptr;
-                        temp _graph (pointer_val_val graph_ptr))
-                 SEP (data_at Tsh
-                              (tarray tint SIZE)
-                              (map Vint (map Int.repr prev'))
-                              (pointer_val_val prev_ptr);
-                      data_at Tsh
-                              (tarray tint SIZE)
-                              (map Vint (map Int.repr priq')) priq_ptr;
-                      data_at Tsh
-                             (tarray tint SIZE)
-                             (map Vint (map Int.repr dist'))
-                             (pointer_val_val dist_ptr);
-                     DijkGraph sh CompSpecs g (pointer_val_val graph_ptr))).
+          (dijk_inner_forloop_inv g sh src priq dist_ptr
+                                  prev_ptr priq_ptr graph_ptr).
         -- unfold SIZE; rep_lia.
         -- (* We start the for loop as planned --
               with the old dist and prev arrays,
@@ -1704,82 +1853,37 @@ Proof.
                                      priq) 0) as u.
           clear H15 H16 H17 H18 H19 H20 H21 H22
                 H23 H24 H25 H26 H27 Ppriq_ptr HPpriq_ptr Ppriq_ptr0.
+          
           split3; [| | split3; [| |split3]]; trivial.
           ++ (* We must show inv_popped for all
                 dst that are in range. *)
             intros. subst u.
             apply (inv_popped_add_u g src dst popped prev
                   priq dist); trivial.
+
           ++ intros.
              destruct (Z.eq_dec dst u).
              1: subst dst; ulia.
-             simpl in H16; destruct H16; [lia|].
-             intro.
-             
+             simpl in H16; destruct H16; [lia | intro].
              destruct (H1 dst) as [? _]; trivial.
-             specialize (H18 H16).
-             destruct H18 as [[? ?] | [src2dst [? [? ?]]]].
-             2: destruct H18 as [? [? [? [? ?]]]]; lia.
+             destruct (H18 H16) as [[? ?] | [src2dst [? [? ?]]]].
+             2: destruct H19 as [? [? [? [? ?]]]]; lia.
              assert (vvalid g u). {
                apply (vvalid_meaning g); trivial; lia.
              }
-             destruct (H19 u H20).
-             specialize (H22 H13). ulia.
+             destruct (H20 u H21).
+             specialize (H23 H13). ulia.
           
-          ++ (* ... in fact, any vertex that is
-                 "seen but not popped"
-                 is that way without the benefit of u.
+          ++ intros.
+             apply (vvalid_meaning g) in H15.
+             apply inv_unpopped_weak_add_unpopped; trivial.
+     
+          ++ intros.
+             apply (vvalid_meaning g) in H15.
+             apply (inv_unseen_weak_add_unpopped g prev _ _ src); trivial.
 
-                 We will be asked to provide a locally optimal
-                 path to such a dst, and we will simply provide the
-                 old one best-known path
-              *)
-            unfold inv_unpopped_weak. intros.
-            apply not_in_cons in H16; destruct H16 as [_ ?].
-            rewrite <- (vvalid_meaning g) in H15; trivial.
-            destruct (H1 dst H15) as [_ [? _]].
-            specialize (H18 H16 H17) as
-                [? | [? [? [? [? [? [? ?]]]]]]]; [left | right]; trivial.
-            
-            unfold V in *.
-            remember (Znth dst prev) as mom.
-
-            assert (evalid g (mom, dst)). {
-                rewrite (evalid_meaning g). split.
-                apply (edge_representable).
-                intro. rewrite <- H25 in H21.
-                apply Zlt_not_le in H21.
-                apply H21; reflexivity.
-            }
-
-            assert (Znth mom dist < inf) by
-                (pose proof (valid_edge_bounds g _ H25); ulia).
-            
-            destruct (popped_noninf_has_path H1 H20 H26) as [p2mom [? [? ?]]]; trivial.
-            
-            (* Several of the proof obligations
-               fall away easily, and those that remain
-               boil down to showing that
-               u was not involved in this
-               locally optimal path.
-             *)
-            assert (mom <> u). {
-              intro contra. rewrite contra in *. apply H13; trivial. 
-            }
-
-            split3; [|split3; [| |split3; [| |split]]|]; trivial.
-            1: simpl; right; trivial.
-            intros.
-            apply H24; trivial.
-            simpl in H33; destruct H33; trilia.
-          ++ unfold inv_unseen_weak. intros.
-             assert (e: dst <> u) by (simpl in H16; lia).
-             apply not_in_cons in H16; destruct H16 as [_ ?].
-             rewrite <- (vvalid_meaning g) in H15; trivial.
-             destruct (H1 dst H15) as [_ [_ ?]].
-             apply H21; trivial.
-             simpl in H19; destruct H19; [lia | trivial].
           ++ apply in_eq.
+
           ++ intros.
              assert (dst <> u). {
                intro. subst dst. apply H16, in_eq.
@@ -1791,48 +1895,59 @@ Proof.
              apply H4; trivial.
              apply not_in_cons in H16; destruct H16 as [_ ?].
              trivial. ulia.
+
           ++ apply Forall_upd_Znth; trivial.
              ulia. rewrite inf_eq; rep_lia.
 
         -- (* We now begin with the for loop's body *)
-          assert (Zlength (@graph_to_mat SIZE g id) = SIZE). {
-            rewrite graph_to_mat_Zlength; trivial. lia.
-          }
-          
-          (* assert (0 <= u < Zlength (@graph_to_mat SIZE g id)). { *)
-            (* rewrite graph_to_mat_Zlength; lia. *)
-          (* } *)
-          assert (1 = 1) by trivial.
-
-          assert (Zlength (Znth u (@graph_to_mat SIZE g id)) = SIZE). {
-            rewrite Forall_forall in H0. apply H0. apply Znth_In.
-            ulia.
-          }
+          rewrite <- Hequ.
           freeze FR := (data_at _ _ _ _) (data_at _ _ _ _) (data_at _ _ _ _).
           unfold DijkGraph.
           rewrite (SpaceAdjMatGraph_unfold _ _ id _ _ u).
           2: ulia.
           Intros.
-          
+          rename H16 into H_inv_popped.
+          rename H17 into H16.
+          rename H18 into H_inv_unpopped.
+          rename H19 into H_inv_unpopped_weak.
+          rename H20 into H_inv_unseen.
+          rename H21 into H_inv_unseen_weak.
+          rename H22 into H17.
+          rename H23 into H18.
+          rename H25 into H_priq_dist_link.
+          rename H26 into H19.
+          rename H27 into H20.
+          rename H28 into H21. 
+
           freeze FR2 := (iter_sepcon _ _) (iter_sepcon _ _).
           unfold list_rep.
           assert_PROP (force_val
                          (sem_add_ptr_int tint Signed
-                                          (force_val (sem_add_ptr_int (tarray tint SIZE) Signed (pointer_val_val graph_ptr) (Vint (Int.repr u))))
+                                          (force_val (sem_add_ptr_int (tarray tint 8) Signed (pointer_val_val graph_ptr) (Vint (Int.repr u))))
                                           (Vint (Int.repr i))) = field_address (tarray tint SIZE) [ArraySubsc i] (@list_address SIZE CompSpecs (pointer_val_val graph_ptr) u)). {
             entailer!.
             unfold list_address. simpl.
             rewrite field_address_offset.
             1: rewrite offset_offset_val; simpl; f_equal; rep_lia.
-            destruct H35 as [? [? [? [? ?]]]].
+            destruct H26 as [? [? [? [? ?]]]].
             unfold field_compatible; split3; [| | split3]; simpl; auto.
-          } 
-          forward. thaw FR2.
+          }
+          
+          assert (Htemp1: Zlength (@graph_to_mat SIZE g id) = SIZE). {
+            rewrite graph_to_mat_Zlength; trivial. lia.
+          }
+          
+          assert (Htemp2: Zlength (Znth u (@graph_to_mat SIZE g id)) = SIZE). {
+            rewrite Forall_forall in H0. apply H0. apply Znth_In.
+            ulia.
+          }
+          
+          forward.
+          clear Htemp1 Htemp2 H22.
+          thaw FR2.
           gather_SEP (iter_sepcon _ _) (data_at _ _ _ _) (iter_sepcon _ _).
           rewrite sepcon_assoc.
           rewrite <- (@SpaceAdjMatGraph_unfold SIZE); trivial. thaw FR.
-          clear H32.
-          assert (1 = 1) by trivial.
           remember (Znth i (Znth u (@graph_to_mat SIZE g id))) as cost.
 
           assert (H_i_valid: vvalid g i). {
@@ -1849,7 +1964,7 @@ Proof.
             entailer!. repeat rewrite Zlength_map in *. trivial. }
           
           forward_if.
-          ++ rename H36 into Htemp.
+          ++ rename H26 into Htemp.
              assert (0 <= cost <= Int.max_signed / SIZE). {
                pose proof (edge_representable g (u, i)).
                rewrite Heqcost in *.
@@ -1858,24 +1973,24 @@ Proof.
                intro.
                rewrite inf_eq2 in Htemp.
                do 2 rewrite Int.signed_repr in Htemp; trivial.
-               rewrite <- H37 in Htemp.
+               rewrite <- H27 in Htemp.
                apply Zlt_not_le in Htemp.
                apply Htemp; reflexivity. (* lemma-fy *)
              }
              clear Htemp.
-             assert (evalid g (u,i)). {
+             assert (H_ui_valid: evalid g (u,i)). {
                apply evalid_dijk with (cost := cost);
                  trivial.
              }
              
              assert (0 <= Znth u dist' <= inf). {
                assert (0 <= u < Zlength dist') by lia.
-               apply (Forall_Znth _ _ _ H38) in H31.
+               apply (Forall_Znth _ _ _ H27) in H21.
                assumption.
              }
              assert (0 <= Znth i dist' <= inf). {
                assert (0 <= i < Zlength dist') by lia.
-               apply (Forall_Znth _ _ _ H39) in H31.
+               apply (Forall_Znth _ _ _ H28) in H21.
                assumption.
              }
              assert (0 <= Znth u dist' + cost <= Int.max_signed). {
@@ -1888,62 +2003,60 @@ Proof.
              unfold V, DE in *.
              
              forward. forward. forward_if.
-             ** rename H41 into improvement.
+             ** rename H30 into H_improvement.
                 (* We know that we are definitely
                    going to make edits in the arrays:
                    we have found a better path to i, via u *)
                 
                 assert (~ In i (popped')).
-                {
+                { (* todo: lemma-fy *)
                   (* This useful fact is true because
                      the cost to i was just improved.
                      This is impossible for popped items.
                    *)
                   intro.
-                  destruct (H19 _ H_i_valid H41).
-                  - destruct H42.
-                    destruct (H43 u H_u_valid).
-                    unfold V, DE in *.
-                    ulia.
-                  - apply Zlt_not_le in improvement.
-                    apply improvement.
-                    destruct (H19 _ H_u_valid H27) as [[? ?] | [p2u [? [? ?]]]].
-                    1: ulia.
-                    destruct H43 as [? [? [? [? ?]]]].
-                    destruct H42 as [p2i [? [? ?]]].
-                    destruct H42 as [? [? [? [? ?]]]].
-                    unfold V, E in *. rewrite H48, H54.
-                    
-                    unfold path_globally_optimal in H51.
-                    specialize (H51 (fst p2u, snd p2u +:: (u,i))).
+                  destruct (H_inv_popped _ H_i_valid H30) as [[? ?] | ?].
+                  1: destruct (H32 u H_u_valid); ulia.
+                  apply Zlt_not_le in H_improvement.
+                  apply H_improvement.
+                  destruct (H_inv_popped _ H_u_valid H24) as [[? ?] | [p2u [? [? ?]]]].
+                  1: ulia.
+                  destruct H32 as [? [? [? [? ?]]]].
+                  destruct H31 as [p2i [? [? ?]]].
+                  destruct H31 as [? [? [? [? ?]]]].
+                  unfold V, E in *. rewrite H37, H43.
+                  
+                  unfold path_globally_optimal in H40.
+                  specialize (H40 (fst p2u, snd p2u +:: (u,i))).
 
-                    rewrite path_cost_app_cons in H51; trivial.
-                    rewrite Heqcost.
-                    apply H51.
-                    + apply valid_path_app_cons.
-                      * rewrite <- surjective_pairing; trivial.
-                      * rewrite (surjective_pairing p2u) in H46.
-                        destruct H46; simpl in H46.
-                        ulia.
-                      * apply strong_evalid_dijk; trivial. ulia.
-                    + apply path_ends_app_cons with (a' := src); trivial.
+                  rewrite path_cost_app_cons in H40; trivial.
+                  rewrite Heqcost.
+                  apply H40.
+                  - apply valid_path_app_cons.
+                    + rewrite <- surjective_pairing; trivial.
+                    + rewrite (surjective_pairing p2u) in H35.
+                      destruct H35; simpl in H35.
+                      ulia.
+                    + apply strong_evalid_dijk; trivial. ulia.
+                  - apply path_ends_app_cons with (a' := src); trivial.
                       3: rewrite <- surjective_pairing; trivial.
                       all: rewrite (surjective_pairing p2u) in *;
-                        destruct H46; simpl in H46; trivial.
+                        destruct H35; simpl in H35; trivial.
                 }
                  
                 assert (Htemp : 0 <= i < Zlength dist') by lia.
-                pose proof (Znth_dist_cases i dist' Htemp H31).
+                pose proof (Znth_dist_cases i dist' Htemp H21).
                 clear Htemp.
-                rename H42 into icases.
-                rewrite <- H28 in icases; trivial.
+                rename H31 into icases.
+                rewrite <- H_priq_dist_link in icases; trivial.
 
-                assert (0 <= i < Zlength (map Vint (map Int.repr dist'))) by
-                    (repeat rewrite Zlength_map; lia).
+                (* assert (0 <= i < Zlength (map Vint (map Int.repr dist'))) by *)
+                    (* (repeat rewrite Zlength_map; lia). *)
                 forward. forward. forward.
                 forward; rewrite upd_Znth_same; trivial.
                 1: entailer!.
-                unfold V, DE in *.
+                1,3: repeat rewrite Zlength_map; lia.
+                (* unfold V, DE in *. *)
                 forward_call (priq_ptr, i, (Znth u dist' + cost), priq').
 
 (* Now we must show that the for loop's invariant
@@ -1955,85 +2068,39 @@ Proof.
    to log a new improved path via u 
  *)
                 1: split; trivial; red; rep_lia.
-                clear H42. 
                 Exists (upd_Znth i prev' u).
                 Exists (upd_Znth i priq' (Znth u dist' + cost)).
                 Exists (upd_Znth i dist' (Znth u dist' + cost)).
                 Exists popped'.
-                repeat rewrite <- upd_Znth_map. entailer!.
-                remember (find priq (fold_right Z.min (hd 0 priq) priq) 0) as u.
-                assert (u <> i) by (intro; subst; lia).
-                split3; [| | split3; [| | split3; [| | split3; [| | split]]]]; intros.
-                --- unfold inv_popped; intros.
-                    pose proof (H19 dst H55 H56).
-                    assert (n: dst <> i). {
-                      intro contra.
-                      rewrite contra in *.
-                      apply H41; trivial.
-                    }
-                    assert (0 <= dst < SIZE). {
-                      apply (vvalid_meaning g) in H55; ulia.
-                    }
-                    repeat rewrite upd_Znth_diff; try lia.
-                    destruct H57; [exfalso | right].
-                    +++ destruct H57.
-                        specialize (H20 _ H55 H56).
-                        unfold V in *. lia.
-                    +++ destruct H57 as [p2dst [? [? ?]]].
-                        exists p2dst. split3; trivial.
-                        *** 
-                          destruct H57 as [? [? [? [? ?]]]].
-                          split3; [| | split3]; trivial.
-                          1: unfold V in *;
-                            rewrite upd_Znth_diff; lia.
-                          rewrite Forall_forall; intros.
-                          assert (In_path g (snd x) p2dst). {
-                            unfold In_path. right.
-                            exists x. split; trivial.
-                            right.
-                            rewrite (edge_dst_snd g); trivial.
-                          }
+                repeat rewrite <- upd_Znth_map.
+                unfold V, DE in *.
+                entailer!.
 
-                          specialize (H59 _ H66).
-                          rewrite Forall_forall in H64.
-                          specialize (H64 _ H65).
-                          destruct H59.
-                          assert (snd x <> i). {
-                            intro contra.
-                            unfold V in *.
-                            rewrite contra in *.
-                            apply H41; trivial; lia.
-                          }
-                          unfold V in *.
-                          rewrite upd_Znth_diff; try lia.
-                          replace (Zlength prev') with SIZE by lia.
-                          rewrite <- (vvalid_meaning g); trivial.
-                          apply (valid_path_valid _ p2dst); trivial.
-                        ***
-                          unfold path_in_popped. intros.
-                          specialize (H59 _ H61).
-                          destruct H59.
-                          assert (step <> i). {
-                            intro contra.
-                            subst step.
-                            apply H41; trivial; lia.
-                          }
-                          split; trivial.
-                          rewrite upd_Znth_diff; trivial.
-                          replace (Zlength dist') with SIZE by lia.
-                          rewrite <- (vvalid_meaning g); trivial.
-                          destruct H57.
-                          apply (valid_path_valid _ p2dst); trivial.
-                          lia.
-                    +++ unfold V in *; lia.
-                    +++ unfold V in *; lia.
-                --- 
-                  destruct (Z.eq_dec dst i).
+                clear H31 H32 H33 H34 H35 H36
+                      H37 H38 H39 H40 H41 H42
+                      HPpriq_ptr Ppriq_ptr Ppriq_ptr0.
+
+                remember (find priq (fold_right Z.min (hd 0 priq) priq) 0) as u.
+                
+                Set Printing All.
+                remember (Znth u dist' + elabel g (u, i)) as newcost.
+                unfold V, DE in *.
+                
+                rewrite <- Heqnewcost in *.
+                Unset Printing All.
+
+                assert (u <> i) by (intro; subst; lia).
+                
+                split3; [| | split3; [| | split3; [| | split3; [| | split]]]]; intros.
+                (* 10 goals, where the 10th is 
+                   3 range-based goals together *)
+                --- apply inv_popped_newcost; trivial.
+                --- destruct (Z.eq_dec dst i).
                     1: subst dst; rewrite upd_Znth_same; trivial; lia.
                     rewrite upd_Znth_diff.
-                    apply H20; trivial.
-                    all: trivial; try lia.
-                    apply (vvalid_meaning g) in H55; ulia.
+                    apply H16; trivial.
+                    apply (vvalid_meaning g) in H32.
+                    all: ulia.
                 --- intros.
                     destruct (Z.eq_dec dst i).
                     +++ subst dst.
@@ -2054,7 +2121,7 @@ Proof.
                           apply (vvalid_meaning g); ulia.
                         }
                         
-                        destruct (H19 _ Hu H27).
+                        destruct (H_inv_popped _ Hu H27).
                         1: unfold V in *; lia.
                         clear H57.
                         unfold V in *.
@@ -2085,7 +2152,7 @@ Proof.
                             }
                             rename H61 into Hk.
                             
-                            destruct (H19 _ H57 H59); trivial.
+                            destruct (H_inv_popped _ H57 H59); trivial.
                             1: unfold V in *; lia.
 
                             
@@ -2426,7 +2493,7 @@ Proof.
                       pose proof (edge_cost_pos g (mom', i)).
                       ulia.
                     }
-                    destruct (H19 _ H64 H65); [unfold V in *; ulia|].
+                    destruct (H_inv_popped _ H64 H65); [unfold V in *; ulia|].
                     
                     destruct H66 as [p2mom' [? [? ?]]].
                     assert (Hrem := H66).
@@ -2626,7 +2693,7 @@ Proof.
           entailer!.
           remember (find priq (fold_right Z.min (hd 0 priq) priq) 0) as u.
           unfold dijkstra_correct.
-          split3; [auto | apply H17 | apply H19];
+          split3; [auto | apply H17 | apply H_inv_popped];
             try rewrite <- (vvalid_meaning g); trivial.
       * (* After breaking from the while loop,
            prove break's postcondition *)
